tests/test_base.thy
@@ -1,0 +1,9 @@
+theory test_base
+  imports "../jeha" SpecCheck.SpecCheck
+begin
+
+text \<open>SpecCheck term generators, etc.\<close>
+
+ML_file\<open>test_base.ML\<close>
+
+end
